SSA/Experimental/Bits/AutoStructs/Tactic.lean
@@ -16,20 +16,7 @@ open Lean Elab Tactic
 open Lean Meta
 open scoped Qq
 
-def AutoStructs.Term.toExpr (t : Term) : Expr :=
-  open Term in
-  match t with
-  | .var n => mkApp (mkConst ``var) (mkNatLit n)
-  | .zero => mkConst ``zero
-  | .one => mkConst ``one
-  | .negOne => mkConst ``negOne
-  | .and t1 t2 => mkApp2 (mkConst ``Term.and) t1.toExpr t2.toExpr
-  | .or t1 t2 => mkApp2 (mkConst ``Term.or) t1.toExpr t2.toExpr
-  | .xor t1 t2 => mkApp2 (mkConst ``Term.xor) t1.toExpr t2.toExpr
-  | .add t1 t2 => mkApp2 (mkConst ``add) t1.toExpr t2.toExpr
-  | .sub t1 t2 => mkApp2 (mkConst ``sub) t1.toExpr t2.toExpr
-  | .not t => mkApp (mkConst ``Term.not) t.toExpr
-  | .neg t => mkApp (mkConst ``neg) t.toExpr
+def AutoStructs.Term.toExpr (t : _root_.Term) : Expr := t.quote
 
 def AutoStructs.Relation.toExpr (rel : Relation) : Expr :=
   open Relation in
@@ -79,7 +66,7 @@ deriving Inhabited
 
 abbrev M := StateRefT State MetaM
 
-def addAsVar (e : Expr) : M AutoStructs.Term := do
+def addAsVar (e : Expr) : M _root_.Term := do
   if let some v ← (←get).varMap.find? e then
       pure (.var v)
   else
@@ -97,18 +84,18 @@ def checkBVs (es : List Expr) : M Bool := do
   pure true
 
 -- TODO: make the shortcuts better
-partial def parseTerm (e : Expr) : M AutoStructs.Term := do
+partial def parseTerm (e : Expr) : M _root_.Term := do
   match_expr e with
   | OfNat.ofNat α n _ =>
     let_expr BitVec _ ← α | addAsVar e
     match n with
-    | .lit (.natVal 0) => pure AutoStructs.Term.zero
-    | .lit (.natVal 1) => pure AutoStructs.Term.one
+    | .lit (.natVal 0) => pure _root_.Term.zero
+    | .lit (.natVal 1) => pure _root_.Term.one
     | _ =>  logWarning m!"Unknown integer {n}"; addAsVar e -- TODO: all other integers...
   | BitVec.ofNat _w n =>
     match n.nat? with
-    | some 0 => pure AutoStructs.Term.zero
-    | some 1 => pure AutoStructs.Term.one
+    | some 0 => pure _root_.Term.zero
+    | some 1 => pure _root_.Term.one
     | _ =>  logWarning m!"Unknown integer {n}"; addAsVar e -- TODO: all other integers...
   | HXor.hXor α1 α2 α3 _ e1 e2 =>
     let_expr BitVec _ ← α1 | addAsVar e
